src/Bedrock/Field/Synthesis/New/Signature.v
@@ -12,6 +12,7 @@ Require Import bedrock2.Semantics.
 Require Import bedrock2.SepAutoArray.
 Require Import bedrock2.Syntax.
 Require Import bedrock2.WeakestPreconditionProperties.
+Require Import bedrock2.ZnWords.
 Require Import coqutil.Byte.
 Require Import coqutil.Map.Interface.
 Require Import coqutil.Tactics.Tactics.
@@ -31,6 +32,7 @@ Require Import Crypto.Bedrock.Specs.Field.
 Require Import Crypto.COperationSpecifications.
 Require Import Crypto.Language.API.
 Require Import Crypto.Spec.ModularArithmetic.
+Require Import Crypto.Util.Tactics.DestructHead.
 Import Language.API.Compilers.
 Import ListNotations.
 Import Types.Notations.
@@ -112,20 +114,21 @@ Section WithParameters.
   Local Notation felem_size_in_words := (felem_size_in_words(FieldRepresentation:=field_representation)).
 
   Lemma FElem_array_truncated_scalar_iff1 px x :
+    length x = felem_size_in_words ->
     Lift1Prop.iff1
       (FElem px x)
-      (sep (map:=mem)
-           (emp (map:=mem) (length x = n))
-           (Array.array
+      (Array.array
               (Scalars.truncated_scalar access_size.word)
               (word.of_Z
                  (Z.of_nat (BinIntDef.Z.to_nat (bytes_per_word width))))
-              px (map word.unsigned x))).
+              px (map word.unsigned x)).
   Proof using ok.
-    cbv [FElem Bignum.Bignum field_representation frep].
+    intros felem_length.
+    cbv [FElem field_representation frep].
     rewrite Util.array_truncated_scalar_scalar_iff1.
-    Morphisms.f_equiv. Morphisms.f_equiv. Morphisms.f_equiv.
-    destruct Bitwidth.width_cases as [W|W]; rewrite W; trivial.
+    Morphisms.f_equiv. Morphisms.f_equiv.
+    pose proof Types.word_size_in_bytes_pos.
+    lia.
   Qed.
 
   Lemma FElemBytes_array_truncated_scalar_iff1 pbs bs :
@@ -148,8 +151,8 @@ Section WithParameters.
   Ltac felem_to_array :=
     repeat
       lazymatch goal with
-      | H:context[sep (FElem _ _) _]
-        |- _ => seprewrite_in FElem_array_truncated_scalar_iff1 H
+      | H:context[sep (FElem _ _) _] |- _ => 
+          seprewrite_in FElem_array_truncated_scalar_iff1 H; [rewrite ?bs2ws_felem_length; lia|]
       | H : context [sep (FElemBytes _ _) _] |- _ =>
         seprewrite_in FElemBytes_array_truncated_scalar_iff1 H
       end.
@@ -297,9 +300,9 @@ Section WithParameters.
     | H : context [FElem pout ?old_out]
       |- @Lift1Prop.ex1 (list Z) _ _ _ =>
       exists (map word.unsigned old_out)
-    | H : context [Placeholder pout ?old_out ]
+    | H : context [sepclause_of_map (?old_out$@pout)]
       |- @Lift1Prop.ex1 (list Z) _ _ _ =>
-      seprewrite_in Placeholder_iff_FElem_bytes H; extract_ex1_and_emp_in_hyps;
+      unshelve seprewrite_in (felem_from_bytes) H; [assumption|];
       exists (map word.unsigned (bs2ws (word:=word) (Z.to_nat (bytes_per_word width)) old_out))
     end;
     crush_sep.
@@ -327,6 +330,7 @@ Section WithParameters.
            end.
 
     Ltac solve_length x Hlength := rewrite map_length;
+    rewrite bs2ws_felem_length; [|assumption];
     match goal with
         | H : (FElem _ x * _)%sep _ |- _ => cbv [FElem Bignum.Bignum] in H; sepsimpl_hyps
         | _ => idtac
@@ -403,16 +407,17 @@ Section WithParameters.
         {
           (* lists_reserved_with_initial_context *)
           lists_reserved_simplify pout; try solve_equivalence_side_conditions;
-          try solve_length (bs2ws (word:=word) (Z.to_nat (bytes_per_word width)) out) outbounds_length.
+          solve_length out outbounds_length.
         } }
-      { postcondition_simplify; [ | | ]; cycle -1.
-        { refine (proj1 (Proper_sep_iff1 _ _ _ _ _ _ _) _);
+      { postcondition_simplify; [ | | | ]; cycle -1.
+        1: refine (proj1 (Proper_sep_iff1 _ _ _ _ _ _ _) _);
             [symmetry; eapply FElem_array_truncated_scalar_iff1 | reflexivity | sepsimpl ].
-          2:eassumption.
-          erewrite <-map_length.
+        1, 4: 
+          erewrite <-map_length;
           match goal with H : map word.unsigned _ = API.interp (res _) _ _ |- _ =>
-            rewrite H end.
-          erewrite length_list_Z_bounded_by; eauto using res_bounds; apply repeat_length. }
+            rewrite H end;
+          erewrite length_list_Z_bounded_by; eauto using res_bounds; apply repeat_length. 
+        { eassumption. }
         { (* output correctness *)
           erewrite <-res_eq; auto.
           match goal with H : map word.unsigned _ = API.interp (res _) _ _ |- _ =>
@@ -490,20 +495,20 @@ Section WithParameters.
         { (* lists_reserved_with_initial_context *)
           lists_reserved_simplify pout.
           all: try solve_equivalence_side_conditions.
-          solve_length (bs2ws (word:=word) (Z.to_nat (bytes_per_word width)) out) outbounds_length. } }
-      { postcondition_simplify; [ | | ].
+          solve_length out outbounds_length. } }
+      { postcondition_simplify; [ | | | ].
         { (* output correctness *)
           eapply res_eq; auto. }
-        { (* output bounds *)
+        { rewrite !map_length. apply outbounds_length; auto. }
+        {(* output bounds *)
           cbn [bounded_by field_representation frep] in *.
           erewrite Util.map_unsigned_of_Z, MaxBounds.map_word_wrap_bounded
             by eauto using relax_list_Z_bounded_by.
           eauto. }
         { (* separation-logic postcondition *)
           eapply Proper_sep_iff1;
-            [ solve [apply FElem_array_truncated_scalar_iff1]
+            [ apply FElem_array_truncated_scalar_iff1
             | reflexivity | ].
-          sepsimpl; [ | ].
           { rewrite !map_length. apply outbounds_length; auto. }
           { erewrite Util.map_unsigned_of_Z, MaxBounds.map_word_wrap_bounded
               by eauto using relax_list_Z_bounded_by.
@@ -576,10 +581,16 @@ Section WithParameters.
           erewrite length_list_Z_bounded_by; [| eapply tight_bounds_tighter_than_max, res_bounds].
           cbv [max_bounds]. rewrite repeat_length. rewrite map_length.
           cbv [FElem Bignum.Bignum] in *. sepsimpl. auto.
+        {
+          rewrite bs2ws_felem_length; auto.
+        }
         } }
-      { postcondition_simplify; [ | | ].
+      { postcondition_simplify; [ | | | ].
         { (* output correctness *)
           eapply res_eq; auto. }
+        { rewrite !map_length.
+            erewrite length_list_Z_bounded_by; [| eapply tight_bounds_tighter_than_max, res_bounds].
+            cbv [max_bounds]; rewrite repeat_length; trivial. }
         { (* output bounds *)
           cbn [bounded_by field_representation frep] in *.
           erewrite Util.map_unsigned_of_Z, MaxBounds.map_word_wrap_bounded
@@ -587,9 +598,8 @@ Section WithParameters.
           eauto. }
         { (* separation-logic postcondition *)
           eapply Proper_sep_iff1;
-            [ solve [apply FElem_array_truncated_scalar_iff1]
+            [ apply FElem_array_truncated_scalar_iff1
             | reflexivity | ].
-          sepsimpl; [ | ].
           { rewrite !map_length.
             erewrite length_list_Z_bounded_by; [| eapply tight_bounds_tighter_than_max, res_bounds].
             cbv [max_bounds]; rewrite repeat_length; trivial. }
@@ -663,7 +673,7 @@ Section WithParameters.
           cbn [type.app_curried fst snd].
           apply res_bounds.
           rewrite max_bounds_range_iff.
-          seprewrite_in @FElem_array_truncated_scalar_iff1 H1; extract_ex1_and_emp_in H1.
+          seprewrite_in @FElem_array_truncated_scalar_iff1 H2; auto.
           ssplit; rewrite ?map_length; trivial.
           eapply List.Forall_map, Forall_forall; intros.
           rewrite MakeAccessSizes.bits_per_word_eq_width.
@@ -671,24 +681,24 @@ Section WithParameters.
         { (* lists_reserved_with_initial_context *)
           lists_reserved_simplify pout.
           all:try solve_equivalence_side_conditions;
-          seprewrite_in (FElem_array_truncated_scalar_iff1 pout) H1; extract_ex1_and_emp_in H1; try eassumption.
-          seprewrite_in (FElem_array_truncated_scalar_iff1 px) H1; extract_ex1_and_emp_in H1.
+          seprewrite_in (FElem_array_truncated_scalar_iff1 pout) H2; rewrite ?bs2ws_felem_length; auto.
+          seprewrite_in (FElem_array_truncated_scalar_iff1 px) H2; auto.
           setoid_rewrite max_bounds_range_iff in res_bounds.
-          rewrite (fun x pf => proj1 (res_bounds x pf)), ?map_length; trivial.
+          rewrite (fun x pf => proj1 (res_bounds x pf)), ?map_length; rewrite ?bs2ws_felem_length; trivial.
           ssplit; rewrite ?map_length; trivial.
           eapply List.Forall_map, Forall_forall; intros.
           rewrite MakeAccessSizes.bits_per_word_eq_width.
           eapply Properties.word.unsigned_range. } }
       postcondition_simplify.
       eapply sep_assoc,sep_comm, sep_assoc. eapply Proper_sep_iff1.
-      { eapply FElem_array_truncated_scalar_iff1. }
+      { eapply (FElem_array_truncated_scalar_iff1); auto. }
       { reflexivity. }
       cbn [List.hd] in *. rewrite MakeAccessSizes.bytes_per_word_eq.
       extract_ex1_and_emp_in_goal; ssplit;
         try (use_sep_assumption; cancel; cbv [seps]);
-        seprewrite_in (FElem_array_truncated_scalar_iff1 px) H1; extract_ex1_and_emp_in H1; trivial.
+        trivial.
       Morphisms.f_equiv.
-      rewrite H5.
+      rewrite H7.
       rewrite <-(res_eq x) at 2 by trivial.
       rewrite Util.map_unsigned_of_Z.
       erewrite map_word_wrap_bounded; trivial.
@@ -784,6 +794,7 @@ Section WithParameters.
       autounfold with equivalence pairs;
       rewrite <-?MakeAccessSizes.bytes_per_word_eq;
       sepsimpl; crush_sep; try solve [solve_equivalence_side_conditions].
+      2: {
         change (Z.of_nat (bytes_per access_size.one)) with 1.
          try
           erewrite Util.map_unsigned_of_Z, map_word_wrap_bounded.
@@ -791,12 +802,16 @@ Section WithParameters.
             seprewrite_in (symmetry! @Util.array_truncated_scalar_ptsto_iff1) H.
             ecancel_assumption. }
           { eapply byte_unsigned_within_max_bounds; try rewrite byte_bounds_length; trivial. }
-        { (* lists_reserved_with_initial_context *)
+      }
+      2: { (* lists_reserved_with_initial_context *)
           lists_reserved_simplify pout.
           all: try solve_equivalence_side_conditions.
           solve_length (bs2ws (word:=word) (Z.to_nat (bytes_per_word width)) out) tight_bounds_length.
-        } }
-      { postcondition_simplify; [ | | ].
+        }
+      erewrite Util.map_unsigned_of_Z,MaxBounds.map_word_wrap_bounded
+        by (eapply byte_unsigned_within_max_bounds; eauto). reflexivity.
+      }
+      { postcondition_simplify; [ | | | ].
         { (* output correctness *)
           eapply res_eq; auto. }
         { (* output bounds *)
@@ -804,11 +819,12 @@ Section WithParameters.
           erewrite Util.map_unsigned_of_Z, MaxBounds.map_word_wrap_bounded
             by eauto using relax_list_Z_bounded_by.
           eauto. }
+        {
+        rewrite !map_length; apply tight_bounds_length; auto. }
         { (* separation-logic postcondition *)
           eapply Proper_sep_iff1;
-            [ solve [apply FElem_array_truncated_scalar_iff1]
+            [ apply FElem_array_truncated_scalar_iff1
             | reflexivity | ].
-          sepsimpl; [ | ].
           { rewrite !map_length; apply tight_bounds_length; auto. }
           { erewrite Util.map_unsigned_of_Z, MaxBounds.map_word_wrap_bounded
               by eauto using relax_list_Z_bounded_by.
@@ -946,8 +962,8 @@ Section WithParameters.
           | |- _ /\ _ => eexists
           end;
         change Field.tight_bounds with tight_bounds in *.
-        { seprewrite_in (@Util.array_truncated_scalar_ptsto_iff1) H11; cbn in H11.
-          rewrite H8, res_eq, partition_le_split in *; trivial. }
+        { seprewrite_in (@Util.array_truncated_scalar_ptsto_iff1) H12; cbn in H12.
+          rewrite H9, res_eq, partition_le_split in *; trivial. }
         rewrite <-partition_le_split, <-res_eq; eauto. }
     Qed.
   End ToBytes.
@@ -1018,11 +1034,6 @@ Context
               pose proof Properties.word.unsigned_range. auto.
     Qed.
 
-    Lemma FElem_max_bounds : forall px x m R, (FElem px x * R)%sep m -> list_Z_bounded_by (@max_bounds width n) (map word.unsigned x).
-    Proof.
-      intros. eapply max_bounds_words. cbv [FElem Bignum.Bignum] in H. sepsimpl. eauto.
-    Qed.
-
     Lemma select_znz_correct f :
       f = make_bedrock_func insizes outsizes inlengths res ->
       forall functions, map.get functions select_znz = Some f ->
@@ -1034,8 +1045,8 @@ Context
       cbv [list_selectznz_insizes list_selectznz_outsizes list_selectznz_inlengths].
       cbv beta; intros; subst f. cbv [make_bedrock_func] in *.
       cleanup.
-      pose proof (FElem_max_bounds _ _ _ _ H1) as Hxbounds.
-      pose proof (FElem_max_bounds _ _ _ _ H2) as Hybounds.
+      pose proof (max_bounds_words _ _ H1) as Hxbounds.
+      pose proof (max_bounds_words _ _ H2) as Hybounds.
       match goal with
       | H : ZRange.is_bounded_by_bool _ _ = _ |- _ => rename H into Hbound
       | _ => idtac
@@ -1067,7 +1078,7 @@ Context
             lists_reserved_simplify pout.
             all: try solve_equivalence_side_conditions.
             destruct (bit_range_eq _ Hbound) as [Hbit| Hbit]; rewrite Hbit; simpl; auto; cbv [FElem Bignum.Bignum] in *; sepsimpl;
-            repeat rewrite map_length;
+            repeat rewrite map_length; rewrite bs2ws_felem_length;
             match goal with
               | H : ?n1 = _ |- ?n1 = _ => rewrite H
               | _ => idtac
@@ -1076,11 +1087,9 @@ Context
         postcondition_simplify.
         destruct (bit_range_eq _ Hbound) as [Hbit| Hbit].
             - rewrite Hbit. simpl. eapply Proper_sep_iff1.
-                + apply FElem_array_truncated_scalar_iff1.
+                + apply FElem_array_truncated_scalar_iff1. assumption.
                 + intros; split; intros; eauto.
                 + sepsimpl; try ecancel_assumption.
-                    * erewrite <- map_length. erewrite length_list_Z_bounded_by; eauto.
-                      cbv [max_bounds]. rewrite repeat_length. eauto.
                     * specialize (res_eq x y pc); rewrite Hbit in res_eq; simpl in res_eq.
                       erewrite <- res_eq; eauto; rewrite <- Hbit; simpl in *; eauto.
                       match goal with
@@ -1088,11 +1097,9 @@ Context
                       | _ => idtac
                       end; eauto.
             - rewrite Hbit; simpl; eapply Proper_sep_iff1.
-                + apply FElem_array_truncated_scalar_iff1.
+                + apply FElem_array_truncated_scalar_iff1. assumption.
                 + intros; split; intros; eauto.
                 + sepsimpl; try ecancel_assumption.
-                    * erewrite <- map_length; erewrite length_list_Z_bounded_by; eauto;
-                      cbv [max_bounds]; rewrite repeat_length; eauto.
                     * specialize (res_eq x y pc); rewrite Hbit in res_eq; simpl in res_eq.
                       erewrite <- res_eq; eauto; rewrite <- Hbit; simpl in *; eauto.
                       match goal with
